# Noether's theorem
#noether-theorem #symmetries #bilinear-products #algebras

# Derivation
Let spacetime be parameterized by an arbitrary scalar $\alpha$. Suppose we infinitesimally transform spacetime and consider its variation to first-order,

$x^\sigma = x^\sigma + \epsilon \frac{\delta x^\sigma}{\delta \lambda}$

where $\epsilon$ is an arbitrarily small parameter and $\frac{\delta x^\sigma}{\delta \lambda}$ is a functional derivative of $x^\sigma$. The variation in the field is,

$\delta \phi^M_{\phantom{M} N} = \left( \nabla_\rho \phi^M_{\phantom{M} N} \right) \delta x^\rho$

$= \epsilon \left( \nabla_\rho \phi^M_{\phantom{M} N} \right) \frac{\delta x^\rho}{\delta \lambda}$

$= \epsilon \: \nabla_{\pmb{X}} \phi^M_{\phantom{M} N}$

The functional derivative of the field is therefore,

$\frac{\delta \phi^M_{\phantom{M} N}}{\delta \lambda} = \frac{\delta \phi^M_{\phantom{M} N}}{\epsilon} = \nabla_{\pmb{X}} \phi^M_{\phantom{M} N}$

Now, the variation in the Lagrangian is,

$\delta \mathcal{L} = \frac{\partial \mathcal{L}}{\partial \phi^M_{\phantom{M} N}} \delta \phi^M_{\phantom{M} N} + \frac{\partial \mathcal{L}}{\partial \left( \nabla_\rho \phi^M_{\phantom{M} N} \right)} \nabla_\rho \left( \delta \phi^M_{\phantom{M} N} \right)$

Using the Euler-Lagrange equations and the functional derivative of the field,

$\delta \mathcal{L} = \epsilon \left\{ \left( \nabla_\rho \pi^{\rho \phantom{M} N}_{\phantom{\rho} M} \right) \frac{\delta \phi^M_{\phantom{M} N}}{\delta \lambda} + \pi^{\rho \phantom{M} N}_{\phantom{\rho} M} \nabla_\rho \frac{\delta \phi^M_{\phantom{M} N}}{\delta \lambda} \right\}$

$= \epsilon \: \nabla_\rho \left( \pi^{\rho \phantom{M} N}_{\phantom{\rho} M} \frac{\delta \phi^M_{\phantom{M} N}}{\delta \lambda} \right)$

But,

$\delta \mathcal{L} = \delta x^\rho \nabla_\rho \mathcal{L}$

$=\epsilon \: \frac{\delta x^\rho}{\delta \lambda} \nabla_\rho \mathcal{L}$

$= \epsilon \left[ \nabla_\rho \left( \frac{\delta x^\rho}{\delta \lambda} \mathcal{L} \right) - \mathcal{L} \: \nabla_\rho \frac{\delta x^\rho}{\delta \lambda} \right]$

Therefore,

$\nabla_\rho \left( \pi^{\rho \phantom{M} N}_{\phantom{\rho} M} \frac{\delta \phi^M_{\phantom{M} N}}{\delta \lambda} \right) - \nabla_\rho \left( \frac{\delta x^\rho}{\delta \lambda} \mathcal{L} \right) + \mathcal{L} \: \nabla_\rho \frac{\delta x^\rho}{\delta \lambda} = 0$

$\nabla_\rho \left( \pi^{\rho \phantom{M} N}_{\phantom{\rho} M} \frac{\delta \phi^M_{\phantom{M} N}}{\delta \lambda} - \frac{\delta x^\rho}{\delta \lambda} \mathcal{L} \right) + \mathcal{L} \: \nabla_\rho \frac{\delta x^\rho}{\delta \lambda} = 0$

Let us now integrate the above over a region of spacetime,

$\displaystyle{ \int_V d^4 x \: \left[ \nabla_\rho \left( \pi^{\rho \phantom{M} N}_{\phantom{\rho} M} \frac{\delta \phi^M_{\phantom{M} N}}{\delta \lambda} - \frac{\delta x^\rho}{\delta \lambda} \mathcal{L} \right) \right] + \int_V d^4 x \: \left( \mathcal{L} \: \nabla_\rho \frac{\delta x^\rho}{\delta \lambda} \right) = 0 }$

By the 4-dimensional divergence theorem, the second term is a constant surface term, and we can set,

$\displaystyle{ \int_V d^4 x \: \left[ \nabla_\rho \left( \pi^{\rho \phantom{M} N}_{\phantom{\rho} M} \frac{\delta \phi^M_{\phantom{M} N}}{\delta \lambda} - \frac{\delta x^\rho}{\delta \lambda} \mathcal{L} \right) \right] = 0 }$

Which means,

$\nabla_\rho \left( \pi^{\rho \phantom{M} N}_{\phantom{\rho} M} \frac{\delta \phi^M_{\phantom{M} N}}{\delta \lambda} - \frac{\delta x^\rho}{\delta \lambda} \mathcal{L} \right) = 0$

We have thus found a conserved current for the transformation concerned:
$$
\begin{align}
j^\rho & = \pi^{\rho \phantom{M} N}_{\phantom{\rho} M} \frac{\delta \phi^M_{\phantom{M} N}}{\delta \lambda} - \frac{\delta x^\rho}{\delta \lambda} \mathcal{L} \\
\nabla_\rho j^\rho & = 0
\end{align}
$$

# Energy-momentum tensor
The energy-momentum tensor is the conserved current generated by symmetry of physical laws under infinitesimal translations in space. An infinitesimal translation of space in the direction of a basis vector $\pmb{e}_\sigma$ can be written as:

$x^\rho \pmb{e}_\rho \to x^\rho \pmb{e}_\rho + \epsilon \: \pmb{e}_\rho$

Or in the component form,

$x^\rho \to x^\rho + \epsilon \: \delta^\rho_{\phantom{\rho} \sigma}$

The functional derivative of the field is given by,

$\frac{\delta \phi^M_{\phantom{M} N}}{\delta \lambda} = \nabla_{\pmb{e}_\sigma} \phi^M_{\phantom{M} N}$

$= \nabla_\sigma \phi^M_{\phantom{M} N}$

Plugging these into the conserved current in Noether's theorem, we get,
$$
j^\rho_{\phantom{\rho} \sigma} = \pi^{\rho \phantom{M} N}_{\phantom{\rho} M} \nabla_\sigma \phi^M_{\phantom{M} N} - \delta^\rho_{\phantom{\rho} \sigma} \mathcal{L}
$$
with the set of equations,
$$
\nabla_\rho j^\rho_{\phantom{\rho} \sigma} = 0
$$
We can raise/lower indices in $j^\rho_{\phantom{\rho} \sigma}$ to express it as the standard energy-momentum tensor:
$$
T^{\rho \sigma} = \pi^{\rho \phantom{M} N}_{\phantom{\rho} M} \nabla^\sigma \phi^M_{\phantom{M} N} - \eta^{\rho \sigma} \mathcal{L}
$$

where $\nabla^\sigma = g^{\sigma \alpha} \nabla_\alpha$ .

# Symmetries and algebras
### Noether current
Suppose a transformation of spacetime is represented by a Jacobian $J^{\rho}_{\phantom{\rho} \sigma}$ , parameterized by a vector $\psi^\alpha$ . An infinitesimal transformation can then be constructed as,

$x^\rho \pmb{e}_\rho \to x^\rho \pmb{e}_\rho + J^{\rho}_{\phantom{\rho} \sigma} \left( \epsilon \: \psi^\alpha \right) \pmb{e}_\rho$

$\implies x^\rho \to x^\rho + J^{\rho}_{\phantom{\rho} \sigma} \left( \epsilon \: \psi^\alpha \right)$

Assuming $\psi^\alpha$ is constrained to contain the components of $J^{\rho}_{\phantom{\rho} \sigma}$ , we can use the fact that scaling the components $\psi^\alpha$ also scales $J^{\rho}_{\phantom{\rho} \sigma}$ to assert,

$x^\rho \to x^\rho + \epsilon \: J^{\rho}_{\phantom{\rho} \sigma} \left( \psi^\alpha \right)$

Therefore, the functional derivative of $x^\rho$ can be written as:
$$
\frac{\delta x^\rho}{\delta \lambda} = J^{\rho}_{\phantom{\rho} \sigma} \left( \psi^\alpha \right)
$$
But, a Jacobian linearly parameterized by a vector must be a contraction of the form,

$J^{\rho}_{\phantom{\rho} \sigma} \left( \psi^\alpha \right) = \psi^\alpha B^\rho_{\phantom{\rho} \alpha \sigma}$
$$
\therefore \frac{\delta x^\rho}{\delta \lambda} = \psi^\alpha B^\rho_{\phantom{\rho} \alpha \sigma}
$$
By the definition of tensors as multilinear maps, $B^\rho_{\phantom{\rho} \alpha \sigma}â€‹$ are the components of a [[bilinear-products|bilinear product]], i.e.,

$\pmb{\mathcal{B}} \left( \pmb{e}_\alpha , \pmb{e}_\sigma \right) = B^\rho_{\phantom{\rho} \alpha \sigma} \pmb{e}_\rho$

The ordered pair $\left( \pmb{\mathcal{B}}, \pmb{\psi} \right)$ where $\pmb{\psi}$ is a variable parameterizing a vector space, generates an [[algebras-over-fields|algebra]] on the vector space.

We also have the reverse scenario where an algebra over a vector space corresponds to a symmetry, yielding the Noether current:

$$
j^\rho_{\phantom{\rho} \sigma} = \psi^\alpha \left( B^\xi_{\phantom{\xi} \alpha \sigma} \pi^{\rho \phantom{M} N}_{\phantom{\rho} M} \nabla_\xi \phi^M_{\phantom{M} N} - B^\rho_{\phantom{\rho} \alpha \sigma} \mathcal{L} \right)
$$

If the action $S$ is symmetric under $J^{\rho}_{\phantom{\rho} \sigma} \left( \psi^\alpha \right)$ for all $\psi^\alpha \in V$ where $V$ is some vector space, we must have the following:

$$j^\rho_{\phantom{\rho} \sigma} = B^\xi_{\phantom{\xi} \alpha \sigma} \pi^{\rho \phantom{M} N}_{\phantom{\rho} M} \nabla_\xi \phi^M_{\phantom{M} N} - B^\rho_{\phantom{\rho} \alpha \sigma} \mathcal{L}$$

### Using gamma matrices

From the [[gamma-matrices#Definition|definition of the gamma matrices]],

$$j^\rho_{\phantom{\rho} \sigma} = \pi^{\rho \phantom{M} N}_{\phantom{\rho} M} \gamma_{\sigma \phantom{\xi} \alpha}^{\phantom{\sigma} \xi} \nabla_\xi \phi^M_{\phantom{M} N} - \gamma_{\sigma \phantom{\rho} \alpha}^{\phantom{\sigma} \rho} \mathcal{L}$$
